Use binder_inductive for Pi_cong

thys/Pi_Calculus/Pi_cong.thy
@@ -2,124 +2,50 @@ theory Pi_cong
   imports Commitment
 begin
 
-(* Structural congurence *)
-inductive cong :: "trm \<Rightarrow> trm \<Rightarrow> bool" (infix "(\<equiv>\<^sub>\<pi>)" 40) where
-  "P = Q \<Longrightarrow> P \<equiv>\<^sub>\<pi> Q"
-| "Par P Q \<equiv>\<^sub>\<pi> Par Q P"
-| "Par (Par P Q) R \<equiv>\<^sub>\<pi> Par P (Par Q R)"
-| "Par P Zero \<equiv>\<^sub>\<pi> P"
-| "x \<noteq> y \<Longrightarrow> Res x (Res y P) \<equiv>\<^sub>\<pi> Res y (Res x P)"
-| "Res x Zero \<equiv>\<^sub>\<pi> Zero"
-| "Bang P \<equiv>\<^sub>\<pi> Par P (Bang P)"
-| "x \<notin> FFVars Q \<Longrightarrow> Res x (Par P Q) \<equiv>\<^sub>\<pi> Par (Res x P) Q"
-
-thm cong_def
-
-(* INSTANTIATING THE LSNominalSet LOCALE: *)
-
 type_synonym T = "trm \<times> trm"
 type_synonym V = "var list" 
 
 
-definition Tperm :: "(var \<Rightarrow> var) \<Rightarrow> T \<Rightarrow> T" where 
-"Tperm f \<equiv> map_prod (rrename f) (rrename f)"
+fun Tperm :: "(var \<Rightarrow> var) \<Rightarrow> T \<Rightarrow> T" where 
+  "Tperm f = map_prod (rrename f) (rrename f)"
 
 fun Tsupp :: "T \<Rightarrow> var set" where 
-"Tsupp (e1,e2) = FFVars e1 \<union> FFVars e2"
+  "Tsupp (e1,e2) = FFVars e1 \<union> FFVars e2"
 
-(*
-definition Vmap :: "(var \<Rightarrow> var) \<Rightarrow> V \<Rightarrow> V" where 
-"Vmap \<equiv> map"
+lemma fresh: "\<exists>xx. xx \<notin> Tsupp (t :: trm \<times> trm)"
+  using Tsupp.simps[of "fst t" "snd t"] unfolding prod.collapse
+  by (metis (no_types, lifting) exists_var finite_iff_le_card_var term.Un_bound term.set_bd_UNIV)
 
-fun Vfvars :: "V \<Rightarrow> var set" where 
-"Vfvars v = set v"
-*)
-
-interpretation LSNominalSet where
-Tperm = Tperm and Tsupp = Tsupp
-apply standard unfolding isPerm_def Tperm_def 
-  using small_Un small_def term.card_of_FFVars_bounds
-  apply (auto simp: term.rrename_id0s map_prod.comp term.rrename_comp0s infinite_UNIV) 
-  by blast
-
-definition G :: "var set \<Rightarrow> (T \<Rightarrow> bool) \<Rightarrow> T \<Rightarrow> bool" where
-  "G \<equiv> \<lambda>B p t.
-    (\<exists>P Q. B = {} \<and> fst t = P \<and> snd t = Q \<and> P = Q) \<or>
-    (\<exists>P Q. B = {} \<and> fst t = Par P Q \<and> snd t = Par Q P) \<or>
-    (\<exists>P Q R. B = {} \<and> fst t = Par (Par P Q) R \<and> snd t = Par P (Par Q R)) \<or>
-    (\<exists>P. B = {} \<and> fst t = Par P Zero \<and> snd t = P) \<or>
-    (\<exists>x y P. B = {x, y} \<and> fst t = Res x (Res y P) \<and> snd t = Res y (Res x P) \<and> x \<noteq> y) \<or>
-    (\<exists>x. B = {x} \<and> fst t = Res x Zero \<and> snd t = Zero) \<or>
-    (\<exists>P. B = {} \<and> fst t = Bang P \<and> snd t = Par P (Bang P)) \<or>
-    (\<exists>x Q P. B = {x} \<and> fst t = Res x (Par P Q) \<and> snd t = Par (Res x P) Q \<and> x \<notin> FFVars Q)"
-
-lemma GG_mono: "R \<le> R' \<Longrightarrow> G v R t \<Longrightarrow> G v R' t"
-  unfolding G_def by force
-
-lemma GG_equiv: "isPerm \<sigma> \<Longrightarrow> small B \<Longrightarrow> G B R t \<Longrightarrow> G (image \<sigma> B) (\<lambda>t'. R (Tperm (inv \<sigma>) t')) (Tperm \<sigma> t)"
-  unfolding G_def
-  by (elim disj_forward exE; cases t)
-    (auto simp: Tperm_def isPerm_def term.rrename_comps
-         | ((rule exI[of _ "\<sigma> _"] exI)+, (rule conjI)?, rule refl)
-         | ((rule exI[of _ "\<sigma> _"])+; auto))+
-
-(* same proofs as for transition *)
-lemma finite_Tsupp: "finite (Tsupp t)"
-  using finite_iff_le_card_var small_Tsupp small_def by blast
-
-lemma exists_fresh:
-"\<exists> z. z \<notin> set xs \<and> (\<forall>t \<in> set ts. z \<notin> Tsupp t)"
-proof-
-  have 0: "|set xs \<union> \<Union> (Tsupp ` (set ts))| <o |UNIV::var set|" 
-  unfolding ls_UNIV_iff_finite  
-  using finite_Tsupp by blast
-  then obtain x where "x \<notin> set xs \<union> \<Union> (Tsupp ` (set ts))"
-  by (meson ex_new_if_finite finite_iff_le_card_var 
-    infinite_iff_natLeq_ordLeq var_term_pre_class.large)
-  thus ?thesis by auto
-qed
-
-lemma isPerm_swap: "isPerm (id(x := y, y := x))"
-  by (auto simp: isPerm_def MRBNF_FP.supp_swap_bound infinite_UNIV)
-
-lemma R_forw_subst: "R (x, y) \<Longrightarrow> (\<And>x y. R (x, y) \<Longrightarrow> R (f x, g y)) \<Longrightarrow> z = g y \<Longrightarrow> R (f x, z)"
-  by blast
-
-lemma G_refresh: 
-  assumes "(\<forall>\<sigma> t. isPerm \<sigma> \<and> R t \<longrightarrow> R (Tperm \<sigma> t))"
-  shows "small B \<Longrightarrow> G B R t \<Longrightarrow> \<exists>C. small C \<and> C \<inter> Tsupp t = {} \<and> G C R t"
-unfolding G_def
-(**)isPerm_def conj_assoc[symmetric]
-unfolding ex_push_inwards conj_disj_distribL ex_disj_distrib ex_simps(1,2)[symmetric]
-    ex_comm[where P = P for P :: "_ set \<Rightarrow> _ \<Rightarrow> _"]
-apply (elim disj_forward exE; simp; clarsimp)
-        apply ((((rule exI conjI)+)?, (assumption | rule Inp_refresh Res_refresh usub_refresh arg_cong2[where f=Cmt, OF refl])
-        | (erule (1) R_forw_subst[of R, OF _ assms[unfolded Tperm_def, simplified, rule_format, OF conjI[OF isPerm_swap]]]; simp?)
-        | (cases t; auto simp only: fst_conv snd_conv Tsupp.simps term.set))+) [3]
-  done
-
-interpretation Cong: Induct where 
-Tperm = Tperm and Tsupp = Tsupp and G = G
-apply standard 
-  using GG_mono GG_equiv G_refresh by auto
-
-lemma cong_I: "(t1 \<equiv>\<^sub>\<pi> t2) = Cong.I (t1, t2)"
-  unfolding cong_def Cong.I_def lfp_curry2 apply(rule arg_cong2[of _ _ _ _ lfp], simp_all)
-  unfolding fun_eq_iff G_def apply clarify
-  subgoal for R PP QQ apply(rule iffI)
-    subgoal apply(elim disjE exE)
-      subgoal by force
-      subgoal for P Q by force
-      subgoal for P Q R by force
-      subgoal by force
-      subgoal for x y P by (metis fst_conv small_two snd_conv)
-      subgoal by auto
-      subgoal for P by simp
-      subgoal for x P Q by auto
-      done
-    subgoal apply(elim conjE disjE exE)
-             apply force+
-      done
+(* Structural congurence *)
+binder_inductive cong :: "trm \<Rightarrow> trm \<Rightarrow> bool" (infix "(\<equiv>\<^sub>\<pi>)" 40) where
+  "P = Q \<Longrightarrow> P \<equiv>\<^sub>\<pi> Q"
+| "Par P Q \<equiv>\<^sub>\<pi> Par Q P"
+| "Par (Par P Q) R \<equiv>\<^sub>\<pi> Par P (Par Q R)"
+| "Par P Zero \<equiv>\<^sub>\<pi> P"
+| "x \<noteq> y \<Longrightarrow> Res x (Res y P) \<equiv>\<^sub>\<pi> Res y (Res x P)" binds "{x, y}"
+| "Res x Zero \<equiv>\<^sub>\<pi> Zero" binds "{x}"
+| "Bang P \<equiv>\<^sub>\<pi> Par P (Bang P)"
+| "x \<notin> FFVars Q \<Longrightarrow> Res x (Par P Q) \<equiv>\<^sub>\<pi> Par (Res x P) Q" binds "{x}"
+where perm: Tperm supp: Tsupp
+         apply (auto simp: o_def split_beta term.rrename_comps fun_eq_iff isPerm_def
+      small_def term.card_of_FFVars_bounds term.Un_bound) [6]
+  subgoal for \<sigma> R B t
+    apply (cases t)
+    apply simp
+    by (elim disj_forward case_prodE)
+      (auto simp: isPerm_def term.rrename_comps
+        | ((rule exI[of _ "\<sigma> _"] exI)+, (rule conjI)?, rule refl)
+        | ((rule exI[of _ "\<sigma> _"])+; auto))+
+  subgoal premises prems for R B t
+    apply (cases t)
+    apply simp
+    using fresh[of t] prems(2-) unfolding
+      (**)isPerm_def conj_assoc[symmetric] split_beta
+    unfolding ex_push_inwards conj_disj_distribL ex_disj_distrib
+    apply (elim disj_forward exE; simp)
+      apply ((rule exI, rule conjI[rotated], assumption) |
+        (((rule exI conjI)+)?, rule Res_refresh) |
+        (cases t; auto))+
     done
   done
 
@@ -129,141 +55,133 @@ thm cong.induct[of P C \<phi>, no_vars]
 corollary strong_induct_cong[consumes 2]:
   assumes
     par: "\<And>p. small (Psupp p)"
-  and cg: "P \<equiv>\<^sub>\<pi> Q"
-  and rules: "\<And>P Q p. P = Q \<Longrightarrow> \<phi> P Q p"
-"\<And>P Q p. \<phi> (Par P Q) (Par Q P) p"
-"\<And>P Q R p. \<phi> (Par (Par P Q) R) (Par P (Par Q R)) p"
-"\<And>P p. \<phi> (Par P Zero) P p"
-"\<And>x y P p. {x, y} \<inter> Psupp p = {} \<Longrightarrow> x \<noteq> y \<Longrightarrow> \<phi> (Res x (Res y P)) (Res y (Res x P)) p"
-"\<And>x p. x \<notin> Psupp p \<Longrightarrow> \<phi> (Res x Zero) Zero p"
-"\<And>P p. \<phi> (Bang P) (Par P (Bang P)) p"
-"\<And>x Q P p. x \<notin> Psupp p \<Longrightarrow> x \<notin> FFVars Q \<Longrightarrow> \<phi> (Res x (Par P Q)) (Par (Res x P) Q) p"
-shows "\<phi> P Q p"
+    and cg: "P \<equiv>\<^sub>\<pi> Q"
+    and rules: "\<And>P Q p. P = Q \<Longrightarrow> \<phi> P Q p"
+    "\<And>P Q p. \<phi> (Par P Q) (Par Q P) p"
+    "\<And>P Q R p. \<phi> (Par (Par P Q) R) (Par P (Par Q R)) p"
+    "\<And>P p. \<phi> (Par P Zero) P p"
+    "\<And>x y P p. {x, y} \<inter> Psupp p = {} \<Longrightarrow> x \<noteq> y \<Longrightarrow> \<phi> (Res x (Res y P)) (Res y (Res x P)) p"
+    "\<And>x p. x \<notin> Psupp p \<Longrightarrow> \<phi> (Res x Zero) Zero p"
+    "\<And>P p. \<phi> (Bang P) (Par P (Bang P)) p"
+    "\<And>x Q P p. x \<notin> Psupp p \<Longrightarrow> x \<notin> FFVars Q \<Longrightarrow> \<phi> (Res x (Par P Q)) (Par (Res x P) Q) p"
+  shows "\<phi> P Q p"
   apply(subgoal_tac "case (P,Q) of (P, Q) \<Rightarrow> \<phi> P Q p")
   subgoal by simp
-  subgoal using par cg apply(elim Cong.strong_induct[where R = "\<lambda>p (P,Q). \<phi> P Q p"])
-    subgoal unfolding cong_I by simp
-    subgoal for p v t apply(subst (asm) G_def) 
-      unfolding cong_I[symmetric] apply(elim disjE exE)
-      subgoal using rules(1) by force
-      subgoal using rules(2) by force
-      subgoal using rules(3) by force
-      subgoal using rules(4) by force
-      subgoal using rules(5) by force
-      subgoal using rules(6) by force
-      subgoal using rules(7) by force
-      subgoal using rules(8) by force
-      done
+  subgoal using par cg apply(elim cong.strong_induct[where R = "\<lambda>p (P,Q). \<phi> P Q p"])
+    subgoal using cong.alt_def by blast
+    subgoal for p v t
+      apply (cases t)
+      apply simp
+      by (meson disjoint_single rules(1) rules(2) rules(3) rules(4) rules(5) rules(6) rules(7) rules(8))
     done
   done
 
 (* Also inferring equivariance from the general infrastructure: *)
 corollary rrename_cong:
-assumes f: "bij f" "|supp f| <o |UNIV::var set|" 
-and r: "P \<equiv>\<^sub>\<pi> Q" 
-shows "rrename f P \<equiv>\<^sub>\<pi> rrename f Q"
-using assms unfolding cong_I using Cong.I_equiv[of "(P,Q)" f]
-unfolding Tperm_def isPerm_def by auto
+  assumes f: "bij f" "|supp f| <o |UNIV::var set|" 
+    and r: "P \<equiv>\<^sub>\<pi> Q" 
+  shows "rrename f P \<equiv>\<^sub>\<pi> rrename f Q"
+  using assms unfolding cong.alt_def using cong.equiv[of "(P,Q)" f]
+  unfolding Tperm.simps isPerm_def by auto
 
-inductive trans :: "trm \<Rightarrow> trm \<Rightarrow> bool" (infix "(\<rightarrow>)" 30) where
-  "Par (Out x z P) (Inp x y Q) \<rightarrow> Par P (usub Q z y)"
+lemma finite_Tsupp: "finite (Tsupp t)"
+  by (metis FFVars_commit_simps(5) Tsupp.simps finite_FFVars_commit finite_Un prod.collapse)
+
+lemma exists_fresh:
+  "\<exists> z. z \<notin> set xs \<and> (\<forall>t \<in> set ts. z \<notin> Tsupp t)"
+proof-
+  have 0: "|set xs \<union> \<Union> (Tsupp ` (set ts))| <o |UNIV::var set|"
+    unfolding ls_UNIV_iff_finite
+    using finite_Tsupp by blast
+  then obtain x where "x \<notin> set xs \<union> \<Union> (Tsupp ` (set ts))"
+    by (meson ex_new_if_finite finite_iff_le_card_var
+        infinite_iff_natLeq_ordLeq var_term_pre_class.large)
+  thus ?thesis by auto
+qed
+
+lemma R_forw_subst: "R (x, y) \<Longrightarrow> (\<And>x y. R (x, y) \<Longrightarrow> R (f x, g y)) \<Longrightarrow> z = g y \<Longrightarrow> R (f x, z)"
+  by blast
+lemma isPerm_swap: "isPerm (id(x := y, y := x))"
+  by (auto simp: isPerm_def MRBNF_FP.supp_swap_bound infinite_UNIV)
+
+binder_inductive trans :: "trm \<Rightarrow> trm \<Rightarrow> bool" (infix "(\<rightarrow>)" 30) where
+  "Par (Out x z P) (Inp x y Q) \<rightarrow> Par P (usub Q z y)" binds "{y}"
 | "P \<rightarrow> Q \<Longrightarrow> Par P R \<rightarrow> Par P Q"
-| "P \<rightarrow> Q \<Longrightarrow> Res x P \<rightarrow> Res x Q"
+| "P \<rightarrow> Q \<Longrightarrow> Res x P \<rightarrow> Res x Q" binds "{x}"
 | "P \<equiv>\<^sub>\<pi> P' \<Longrightarrow> P' \<rightarrow> Q' \<Longrightarrow> Q' \<equiv>\<^sub>\<pi> Q \<Longrightarrow> P \<rightarrow> Q"
-
-thm trans_def
-
-definition G_trans :: "var set \<Rightarrow> (T \<Rightarrow> bool) \<Rightarrow> T \<Rightarrow> bool" where
-  "G_trans \<equiv> \<lambda>B p t.
-    (\<exists>x z P y Q. B = {y} \<and> fst t = Par (Out x z P) (Inp x y Q) \<and> snd t = Par P (usub Q z y)) \<or>
-    (\<exists>P Q R. B = {} \<and> fst t = Par P R \<and> snd t = Par P Q \<and> p (P, Q)) \<or>
-    (\<exists>P Q x. B = {x} \<and> fst t = Res x P \<and> snd t = Res x Q \<and> p (P, Q)) \<or>
-    (\<exists>P P' Q' Q. B = {} \<and> fst t = P \<and> snd t = Q \<and> (P \<equiv>\<^sub>\<pi> P') \<and> p (P', Q') \<and> (Q' \<equiv>\<^sub>\<pi> Q))"
-
-lemma GG_trans_mono: "R \<le> R' \<Longrightarrow> G_trans v R t \<Longrightarrow> G_trans v R' t"
-  unfolding G_trans_def by blast
-
-lemma GG_trans_equiv: "isPerm \<sigma> \<Longrightarrow> small B \<Longrightarrow> G_trans B R t \<Longrightarrow> G_trans (image \<sigma> B) (\<lambda>t'. R (Tperm (inv \<sigma>) t')) (Tperm \<sigma> t)"
-  unfolding G_trans_def
-  apply (elim disj_forward exE; cases t)
-  apply  (auto simp: Tperm_def isPerm_def term.rrename_comps
-         | ((rule exI[of _ "\<sigma> _"] exI)+, (rule conjI)?, rule refl)
-         | ((rule exI[of _ "\<sigma> _"])+; auto))+
-  by (metis Pi_cong.rrename_cong bij_imp_inv' term.rrename_bijs term.rrename_inv_simps)
-
-lemma G_trans_refresh: 
-  assumes "(\<forall>\<sigma> t. isPerm \<sigma> \<and> R t \<longrightarrow> R (Tperm \<sigma> t))"
-  shows "small B \<Longrightarrow> G_trans B R t \<Longrightarrow> \<exists>C. small C \<and> C \<inter> Tsupp t = {} \<and> G_trans C R t"
-unfolding G_trans_def
-(**)isPerm_def conj_assoc[symmetric]
-  unfolding ex_push_inwards conj_disj_distribL ex_disj_distrib ex_simps(1,2)[symmetric]
-    ex_comm[where P = P for P :: "_ set \<Rightarrow> _ \<Rightarrow> _"]
-  apply (elim disj_forward exE; simp; clarsimp)
-  apply (cases t; auto simp only: fst_conv snd_conv Tsupp.simps term.set)
-  subgoal for x z P y Q
-    apply (rule exE[OF exists_fresh[of "[x, y, z]" "[(P, Q)]"]])
-    subgoal for w
-      apply (rule exI[of _ w])
-      apply simp
-      by (meson Inp_refresh usub_refresh)
-    done
-  apply ((((rule exI conjI)+)?, (assumption | rule Inp_refresh Res_refresh usub_refresh arg_cong2[where f=Cmt, OF refl])
-        | (erule (1) R_forw_subst[of R, OF _ assms[unfolded Tperm_def, simplified, rule_format, OF conjI[OF isPerm_swap]]]; simp?)
-        | (cases t; auto simp only: fst_conv snd_conv Tsupp.simps term.set))+)
-  done
-
-interpretation Trans: Induct where
-Tperm = Tperm and Tsupp = Tsupp and G = G_trans
-apply standard 
-  using GG_trans_mono GG_trans_equiv G_trans_refresh by auto
-
-lemma trans_I: "trans t1 t2 = Trans.I (t1,t2)"
-unfolding trans_def Trans.I_def lfp_curry2 apply(rule arg_cong2[of _ _ _ _ lfp], simp_all)
-  unfolding fun_eq_iff G_trans_def apply clarify
-subgoal for R PP QQ apply(rule iffI)
-  subgoal apply(elim disjE exE)
-    subgoal by fastforce
-    subgoal by force
-    subgoal by force
-    subgoal by force
-    done
-  subgoal apply(elim disjE exE)
-    subgoal by fastforce
-    done
-  done
+where perm: Tperm supp: Tsupp
+         apply (auto simp: o_def split_beta term.rrename_comps fun_eq_iff isPerm_def
+      small_def term.card_of_FFVars_bounds term.Un_bound) [6]
+  subgoal for \<sigma> R B t
+    apply (cases t)
+    apply simp
+    apply (elim disj_forward exE; cases t)
+       apply  (auto simp: isPerm_def term.rrename_comps
+        | ((rule exI[of _ "\<sigma> _"] exI)+, (rule conjI)?, rule refl)
+        | ((rule exI[of _ "\<sigma> _"])+; auto))+
+    by (metis Pi_cong.rrename_cong bij_imp_inv' term.rrename_bijs term.rrename_inv_simps)
+  subgoal premises prems for R B t
+  proof -
+    define G_trans where "G_trans \<equiv> \<lambda>B p t.
+                (\<exists>x z P y Q. B = {y} \<and> fst t = Out x z P \<parallel> Inp x y Q \<and> snd t = P \<parallel> Q[z/y]) \<or>
+                (\<exists>P Q R. B = {} \<and> fst t = P \<parallel> R \<and> snd t = P \<parallel> Q \<and> p (P, Q)) \<or>
+                (\<exists>P Q x. B = {x} \<and> fst t = Res x P \<and> snd t = Res x Q \<and> p (P, Q)) \<or> (\<exists>P P' Q' Q. B = {} \<and> fst t = P \<and> snd t = Q \<and> P \<equiv>\<^sub>\<pi> P' \<and> p (P', Q') \<and> Q' \<equiv>\<^sub>\<pi> Q)"
+    { assume assms: "(\<forall>\<sigma> t. isPerm \<sigma> \<and> R t \<longrightarrow> R (Tperm \<sigma> t))"
+      have "small B \<Longrightarrow> G_trans B R t \<Longrightarrow> \<exists>C. small C \<and> C \<inter> Tsupp t = {} \<and> G_trans C R t"
+        unfolding G_trans_def isPerm_def conj_assoc[symmetric]
+        unfolding ex_push_inwards conj_disj_distribL ex_disj_distrib ex_simps(1,2)[symmetric]
+          ex_comm[where P = P for P :: "_ set \<Rightarrow> _ \<Rightarrow> _"]
+        apply (elim disj_forward exE; simp; clarsimp)
+          apply (cases t; auto simp only: fst_conv snd_conv Tsupp.simps term.set)
+        subgoal for x z P y Q
+          apply (rule exE[OF exists_fresh[of "[x, y, z]" "[(P, Q)]"]])
+          subgoal for w
+            apply (rule exI[of _ w])
+            apply simp
+            by (meson Inp_refresh usub_refresh)
+          done
+         apply ((((rule exI conjI)+)?, (assumption | rule Inp_refresh Res_refresh usub_refresh arg_cong2[where f=Cmt, OF refl])
+              | (erule (1) R_forw_subst[of R, OF _ assms[unfolded Tperm.simps, simplified, rule_format, OF conjI[OF isPerm_swap]]]; simp?)
+              | (cases t; auto simp only: fst_conv snd_conv Tsupp.simps term.set))+)
+        done
+    }
+    then show ?thesis unfolding G_trans_def using prems by force
+  qed
   done
 
 thm trans.induct[of P Q \<phi>, no_vars]
 
 corollary strong_induct_trans[consumes 2]:
   assumes par: "\<And>p. small (Psupp p)"
-  and tr: "trans P Q"
-  and rules:
-  "\<And>x z P y Q p. y \<notin> Psupp p \<Longrightarrow> \<phi> (Par (Out x z P) (Inp x y Q)) (Par P (usub Q z y)) p"
-  "\<And>P Q R p. P \<rightarrow> Q \<Longrightarrow> (\<And>p. \<phi> P Q p) \<Longrightarrow> \<phi> (Par P R) (Par P Q) p"
-  "\<And>P Q x p. x \<notin> Psupp p \<Longrightarrow> P \<rightarrow> Q \<Longrightarrow> (\<And>p. \<phi> P Q p) \<Longrightarrow> \<phi> (Res x P) (Res x Q) p"
-  "\<And>P P' Q' Q p. P \<equiv>\<^sub>\<pi> P' \<Longrightarrow> P' \<rightarrow> Q' \<Longrightarrow> (\<And>p. \<phi> P' Q' p) \<Longrightarrow> Q' \<equiv>\<^sub>\<pi> Q \<Longrightarrow> \<phi> P Q p"
-shows "\<phi> P Q p"
-apply(subgoal_tac "case (P,Q) of (P, Q) \<Rightarrow> \<phi> P Q p")
+    and tr: "trans P Q"
+    and rules:
+    "\<And>x z P y Q p. y \<notin> Psupp p \<Longrightarrow> \<phi> (Par (Out x z P) (Inp x y Q)) (Par P (usub Q z y)) p"
+    "\<And>P Q R p. P \<rightarrow> Q \<Longrightarrow> (\<And>p. \<phi> P Q p) \<Longrightarrow> \<phi> (Par P R) (Par P Q) p"
+    "\<And>P Q x p. x \<notin> Psupp p \<Longrightarrow> P \<rightarrow> Q \<Longrightarrow> (\<And>p. \<phi> P Q p) \<Longrightarrow> \<phi> (Res x P) (Res x Q) p"
+    "\<And>P P' Q' Q p. P \<equiv>\<^sub>\<pi> P' \<Longrightarrow> P' \<rightarrow> Q' \<Longrightarrow> (\<And>p. \<phi> P' Q' p) \<Longrightarrow> Q' \<equiv>\<^sub>\<pi> Q \<Longrightarrow> \<phi> P Q p"
+  shows "\<phi> P Q p"
+  apply(subgoal_tac "case (P,Q) of (P, Q) \<Rightarrow> \<phi> P Q p")
   subgoal by simp
-  subgoal using par tr apply(elim Trans.strong_induct[where R = "\<lambda>p (P,Q). \<phi> P Q p"])
-    subgoal unfolding trans_I by simp
-    subgoal for p v t apply(subst (asm) G_trans_def) 
-      unfolding trans_I[symmetric] apply(elim disjE exE)
+  subgoal using par tr apply(elim trans.strong_induct[where R = "\<lambda>p (P,Q). \<phi> P Q p"])
+    subgoal unfolding trans.alt_def by blast
+    subgoal for p v t
+      apply (cases t)
+      apply simp
+      apply(elim disjE exE)
       subgoal using rules(1) by auto
-      subgoal using rules(2) by auto
-      subgoal using rules(3) by auto
-      subgoal using rules(4) by auto
+      subgoal using rules(2) trans.alt_def[symmetric] by auto
+      subgoal using rules(3) trans.alt_def[symmetric] by auto
+      subgoal using rules(4) trans.alt_def[symmetric] by auto
       done
     done
   done
 
 (* Also inferring equivariance from the general infrastructure: *)
 corollary rrename_trans:
-assumes f: "bij f" "|supp f| <o |UNIV::var set|" 
-and r: "trans P Q" 
-shows "trans (rrename f P) (rrename f Q)"
-using assms unfolding trans_I using Trans.I_equiv[of "(P,Q)" f]
-unfolding Tperm_def isPerm_def by auto
+  assumes f: "bij f" "|supp f| <o |UNIV::var set|" 
+    and r: "trans P Q" 
+  shows "trans (rrename f P) (rrename f Q)"
+  using assms unfolding cong.alt_def using cong.equiv[of "(P,Q)" f]
+  using isPerm_def trans.alt_def trans.equiv by fastforce
 
 end
